## 1

Inicialmente K recebe 0

A cada iteração, K é incrementado em 1, e SOMA é incrementada pelo novo valor de K.

K=1 -> SOMA = 0 + 1 = 1 \
K=2 -> SOMA = 1 + 2 = 3 \
K=3 -> SOMA = 3 + 3 = 6 \
K=4 -> SOMA = 6 + 4 = 10 \
K=5 -> SOMA = 10 + 5 = 15 \
K=6 -> SOMA = 15 + 6 = 21 \
K=7 -> SOMA = 21 + 7 = 28 \
K=8 -> SOMA = 28 + 8 = 36 \
K=9 -> SOMA = 36 + 9 = 45 \
K=10 -> SOMA = 45 + 10 = 55 \
K=11 -> SOMA = 55 + 11 = 66 \
K=12 -> SOMA = 66 + 12 = 78 \
K=13 -> SOMA = 78 + 13 = 91 \

O valor de soma será 91